
\chapter{Inferring Clause Type from Syntax, Prosody, Speech Act}
\label{appx:eng-model-dir}

\begin{figure}[H]
\begin{center}
\begin{tikzpicture}
\node[obs] (a) {$A_{i}$};
\node[latent, below=of a] (c) {$C_{i}$};
\node[obs, below=of c, xshift=-0.6cm] (s) {$\vec{S_{i}}$};
\node[obs, below=of c, xshift=0.6cm] (l) {$L_{i}$};
%\node[latent, right=of l] (lambda) {$\lambda^{c}$};
%\node[obs, right=of lambda] (eta) {$\eta$};
\node[latent, right=of c] (phi) {$\phi^{a}$};
\node[obs, right=of phi] (beta) {$\beta$};
%\node[latent, left=of s] (delta) {$\delta^{c}$};
%\node[obs, left=of delta] (gamma) {$\gamma$};

\edge {phi, a}{c};
\edge {c}{s};
\edge {beta}{phi};
%\edge {gamma}{delta};
\edge {c}{l};
%\edge {eta}{lambda};


\plate {avalue}{(phi)}{$A$};
%\plate {cvalue}{(delta)}{$C$};
\plate {fvalue}{(s)}{$F$};
\plate {nutt}{(a)(c)(s)(l)(fvalue)}{$N$};
\end{tikzpicture}
\end{center}
\caption{Hierarchical model}\label{fig:appx-baseline}
\end{figure}

Variables:
\begin{itemize}
\item A: Speech Act, four values: Assertion, Question, Request/Command, other%\\
%$ a \sim \mbox{Multinomial}(\vec{\theta})$;\\
%$\vec{\theta} \sim \mbox{Dir}(\alpha)$
\item C: Clause Type, four values: declarative, interrogative, imperative, other\\
$ c \sim \mbox{Multinomial}(\vec{\phi^{a}})$;\\
$\vec{\phi^{a}} \sim \mbox{Dir}(\beta)$
\item $\vec{S}$: Syntactic features, feature bundle; 
the value of each feature $F$ is $S^{(F)}$ \\
$s^{(F)} \sim \mbox{Bernoulli}(\delta^{c})$ \\
$\delta\sim \mbox{Beta}(\gamma)$
\item $L$: Intonation; rise or otherwise\\
$l\sim\mbox{Bernoulli}(\lambda^{c}) $\\
$\lambda^{c}\sim\mbox{Beta}(\eta)$
%\item $\vec{R}$: proportion of looks before, during, and after an utterance\\
%$\vec{R_{i}} \sim \mbox{MVN}(\mu_{A}, \Sigma_{A})$ 
\end{itemize}

%For utterances \{1, \ldots, n\}:
%\begin{equation}
%P(C | A, S) = P(S|C) P(C) P(C|A) 
%\end{equation}

\begin{figure}[H]
\begin{center}
\begin{tikzpicture}
\node[obs] (a) {$A_{i}$};
\node[latent, below=of a] (c) {$C_{i}$};
\node[obs, below=of c, xshift=-0.6cm] (s) {$\vec{S_{i}}$};
\node[obs, below=of c, xshift=0.6cm] (l) {$L_{i}$};
\node[latent, right=of l] (lambda) {$\lambda^{c}$};
\node[obs, right=of lambda] (eta) {$\eta$};
\node[latent, right=of c] (phi) {$\phi^{a}$};
\node[obs, right=of phi] (beta) {$\beta$};
\node[latent, left=of s] (delta) {$\delta^{c}$};
\node[obs, left=of delta] (gamma) {$\gamma$};

\edge {phi, a}{c};
\edge {delta, c}{s};
\edge {beta}{phi};
\edge {gamma}{delta};
\edge {c,lambda}{l};
\edge {eta}{lambda};


\plate {nutt}{(a)(c)(s)(l)}{$N$};
\plate {avalue}{(phi)}{$A$};
\plate {cvalue}{(delta)}{$C$};
\plate {fvalue}{(gamma)(delta)(s)(cvalue)}{$F$};
\end{tikzpicture}
\end{center}
\caption{Hierarchical model with all parameters specified}\label{fg:model}
\end{figure}

\subsection{Notations}
\begin{itemize}
\item $c_{i}$: value of variable $C$ for utterance $i$
\item $c_{-i}$: value of variable $C$ for utterances other than $i$
\item $\vec{c}$: value of variable $C$ for all utterances
%\item $c_{i}'$: all possible values of $c$
\item $S_{i}$: values of all syntactic features for $i$
\item $s^{(F)}_{i}$: the value of syntactic feature $s^{F}$ for $i$
\item $l_{i}$: value of variable $L$ for utterance $i$ (rise or otherwise)
\item $n$: total number of utterances
\item $n_{c_{i}}$: number of observations where $c=c_{i}$
\item $n^{(c_{i}, F)}_{s_{i}}$ is the number of observations where the value of feature $s^{F} = s^{F}_{i}$ and $c = c_{i}$ 
\item $n^{(F)}_{c_{i}}$ is the number of total observations of feature $s^{F}$ so far when $c = c_{i}$. 
\item $n^{c_{i}}_{l_{i}}$: the number of observations where $L = l_{i}$ and $c = c_{i}$
\end{itemize}

\subsection{Sampling C}
\begin{equation}
p(c_{i}| c_{-i}, \vec{a}, \beta, \vec{S_{i}}, \delta, \gamma, l_{i}, \lambda, \eta) = \frac{p(\vec{S_{i}}| \vec{c}, \delta, \gamma)\ p(l_{i} |\vec{c},\lambda, \eta)\ p(c_{i}|\beta, c_{-i}, \vec{a})}{\Sigma_{c_{i}'}p(\vec{S_{i}}| \vec{c'}, \delta, \gamma)\ p(l_{i} |\vec{c'},\lambda, \eta)\ p(c_{i}'|\beta, c_{-i}, \vec{a})}
\end{equation}

\subsubsection{Likelihood}
Each syntactic feature $s^{(F)}\sim \mbox{Bernoulli}(\delta_{c})$. Assume that $n^{(F)}_{s_{i}}$ is the number of observations where $s^{(F)}_{i}=s_{i}$ when $c=c_{i}$, and $n_{c_{i}}$ is the number of total observations of $s^{(F)}$ when $c=c_{i}$. The feature superscript $(F)$ is omitted from line 4 forward for simplicity.

\begin{equation}
\begin{split}\label{p(s|c)}
p(\vec{S_{i}}| \vec{c}, \delta, \gamma) = & \prod_{F} p(s^{(F)}_{i}|\vec{c}^{(F)}, \delta, \gamma)\\%split to each feature of S
= &\prod_{F}\int p(s^{(F)}_{i}|c_{i}^{(F)}, \delta^{(F)}_{c_{i}}, \gamma^{(F)})\ p(\delta^{(F)}_{c_{i}}|c^{(F)}_{-i}, s^{(F)}_{-i},\gamma^{(F)}) d\delta_{c_{i}}\\%predicative posterior distribution
=& \prod_{F}\int \prod_{k} \delta^{1^{s_{i}=k}}_{k}%expand p(s_{i})
\prod_{k} \delta_{k}^{\gamma_{k}-1}  %expand p(delta)
\frac{\Gamma(\sum_{k}(\gamma_{k}))}{\prod_{k}(\Gamma(\gamma_{k}))}%normalizing constant for p(delta)
d\delta_{c_{i}} \\ 
=& \prod_{F} \frac{\Gamma(\sum_{k}(\gamma_{k}))}{\prod_{k}(\Gamma(\gamma_{k}))}%move the normalizing constant 
\int \prod_{k}\delta_{k}^{1^{s_{i}=k}+\gamma_{k}-1}d\delta_{c_{i}} %combine the two deltas and (1-delta)s
\end{split}
\end{equation}

\noindent The last term could be solved by adding a constant to create the PDF of the following Beta distribution (with parameter $\gamma_{k}+1^{s_{i}=k} $):
\begin{equation}
\begin{split}
&p(\delta_{c_{i}}|\gamma_{k}+1^{s_{i}=k})\\
=&\int \prod_{k}\delta_{k}^{1^{s_{i}=k}+\gamma_{k}-1}%delta terms
\frac{\Gamma(\sum_{k}(\gamma_{k}+1^{s_{i}=k}))}{\prod_{k}(\Gamma(\gamma_{k}+1^{s_{i}=k}))}%normalizing constant with new parameter
d\delta_{c_{i}}
\end{split}
\end{equation}


Therefore Equation (\ref{p(s|c)}) can be rewritten as:
\begin{equation}
\begin{split}
p(\vec{S_{i}}| \vec{c}, \delta, \gamma)
= & \prod_{F} \frac{\Gamma(\sum_{k}(\gamma_{k}))}{\prod_{k}(\Gamma(\gamma_{k}))}%normalizing constant 
\int \prod_{k}\delta_{k}^{1^{s_{i}=k}+\gamma_{k}-1}d\delta_{c_{i}}\\
=&\prod_{F} \frac{\Gamma(\sum_{k}(\gamma_{k}))}{\prod_{k}(\Gamma(\gamma_{k}))}%old NC
\frac{\prod_{k}(\Gamma(\gamma_{k}+1^{s_{i}=k}))}{\Gamma(\sum_{k}(\gamma_{k}+1^{s_{i}=k}))} %1/new NC
\int \prod_{k}\delta_{k}^{1^{s_{i}=k}+\gamma_{k}-1}
\frac{\Gamma(\sum_{k}(\gamma_{k}+1^{s_{i}=k}))}{\prod_{k}(\Gamma(\gamma_{k}+1^{s_{i}=k}))}%pdf of Beta(gamma+1^{si=k})
d\delta_{c_{i}}\\
=&\prod_{F} \frac{\Gamma(\sum_{k}(\gamma_{k}))}{\prod_{k}(\Gamma(\gamma_{k}))}%old NC
\frac{\prod_{k}(\Gamma(\gamma_{k}+1^{s_{i}=k}))}{\Gamma(\sum_{k}(\gamma_{k}+1^{s_{i}=k}))}\\ %1/new NC
=&\prod_{F}\frac{\Gamma(\sum_{k}(\gamma_{k}))}{\Gamma(\gamma_{s_{i}})\prod_{k\neq s_{i}}(\Gamma(\gamma_{k}))}%old NC
\frac{\Gamma(\gamma_{s_{i}}+1)\prod_{k\neq s_{i}}(\Gamma(\gamma_{k}))}{\Gamma(\sum_{k}(\gamma_{k})+1)}\\%separate out k from s_{i}
=&\prod_{F}\frac{\gamma_{s_{i}}}{\sum_{k}(\gamma_{k})}\\%reduce
=&\prod_{F}\frac{\gamma_{0}+n_{s_{i}}}{(r_{0}+n_{s_{i}})(r_{0}+n_{c_{i}}-n_{s_{i}})}\\%update function
=& \prod_{F}\frac{\gamma_{0}+n_{s^{F, c_{i}}_{i}}}{2r_{0}+n^{F}_{c_{i}}}
\end{split}
\end{equation}

Similarly for L:
\begin{equation}
\begin{split}
p(l_{i} |\vec{c},\lambda, \eta) &= \frac{\eta_{l_{i}}}{\sum_{k}{\eta_{k}}}\\
&= \frac{\eta_{0}+n_{l_{i}}^{c_{i}}}{2\eta_{0}+n_{c_{i}}}
\end{split}
\end{equation}

\subsubsection{Prior}
Assume $\beta_{k}$ is the value of $\beta$ for when $c = k$, $n_{c_{i}}$ as the number of observations of $c=c_{i}$ so far, and  $n_{c_{i}}^{(k)}$ is the number of observations of other values of $c$ 
%p(c_{i}|\phi_{a_{i}},a_{i}) = \prod_{k}\phi_{a_{i}} 

\begin{equation}
\begin{split}
 p(c_{i}|\phi_{a_{i}} ,\beta, c_{-i},  \vec{a})  =& \int p(c_{i}|\phi_{a_{i}}, \beta) p(\phi_{a_{i}}| c_{-i}, \beta)d\phi_{a_{i}} \\
= & \int \prod_{k}\ \phi_{k}^{1^{c_{i}=k}}\ \frac{\Gamma(\sum_{k}\beta_{k})}{\prod_{k}(\Gamma(\beta_{k}))}\prod_{k} \phi_{k}^{\beta_{k}-1}d\phi\\
= & \ \frac{\Gamma(\sum_{k}\beta_{k})}{\prod_{k}(\Gamma(\beta_{k}))} %dirchlet
\frac{\prod_{k\neq c_{i}}\Gamma(\beta_{k})\Gamma (\beta_{c_{i}}+1)}{\Gamma(\sum_{k}\beta_{k} +1)} \, %norm constant^{-1}
\int \prod_{k\neq c_{i}} \phi_{k}^{\beta_{k}-1} \phi_{c_{i}}^{\beta_{c_{i}}}\ %integral
\frac{\Gamma(\sum_{k}\beta_{k}+1)}{\prod_{k\neq c_{i}} (\Gamma(\beta_{k}) \Gamma(\beta_{c_{i}}+1))} d\phi\\%norm constant inside and out
= &  \frac{\Gamma(\sum_{k}\beta_{k})}{\prod_{k}(\Gamma\beta_{k})}\ %dirchlet
\frac{\prod_{k\neq c_{i}}\Gamma(\beta_{k})\Gamma (\beta_{c_{i}}+1)}{\Gamma(\sum_{k}\beta_{k} +1)} \, %norm constant^{-1}
\int \prod_{k\neq c_{i}} \phi_{k}^{\beta_{k}-1} \phi_{c_{i}}^{\beta_{c_{i}}}%integral
\frac{\Gamma(\sum_{k}\beta_{k} +1)}{\prod_{k\neq c_{i}} (\Gamma(\beta_{k}) \Gamma(\beta_{c_{i}}+1))} \  %norm constant
d\phi\\
=&\frac{\Gamma(\sum_{k}\beta_{k})}{\prod_{k}(\Gamma\beta_{k})}%dirchlet 
\frac{\prod_{k\neq c_{i}} (\Gamma(\beta_{k}) \Gamma(\beta_{c_{i}}+1)}{\Gamma(\sum_{k}\beta_{k}+1)} \\%reduction
= &\frac{\beta_{c_{i}}}{\sum_{k}(\beta_{k})}\\
= & \frac{\beta_{0}+n_{c_{i}}^{a_{i}}}{\sum_{k}(\beta_{0}+n^{(k,a_{i})}_{c_{i}})}\\
= & \frac{\beta_{0}+n_{c_{i}}^{a_{i}}}{4\beta_{0}+n_{a_{i}}}
\end{split}
\end{equation}


%\begin{comment}
\subsubsection{Posterior distribution of $c$}
The posterior probability distribution of $c$ of value $i$ is calculated by computing the product of the prior of $c$ given every other variables and the likelihood, and normalized by dividing the sum of the posterior of $c$ of every value

\begin{equation}\label{postC}
\begin{split}
p(c_{i}| c_{-i}, \vec{a}, \beta, \vec{S_{i}}, \delta, \gamma, l_{i}, \lambda, \eta) = &
\frac{p(\vec{S_{i}}| \vec{c}, \delta, \gamma)\ p(l_{i} |\vec{c},\lambda, \eta)\ p(c_{i}|\beta, c_{-i}, \vec{a})}{\Sigma_{c_{i}'}p(\vec{S_{i}}| \vec{c'}, \delta, \gamma)\ p(l_{i} |\vec{c'},\lambda, \eta)\ p(c_{i}'|\beta, c_{-i}, \vec{a})}\\
=& \frac{ \prod_{F}\frac{\gamma_{0}+n_{s^{F, c_{i}}_{i}}}{2r_{0}+n_{c^{F}_{i}}}%S
\frac{\eta_{0}+n_{l_{i}}^{c_{i}}}{2\eta_{0}+n_{c_{i}}}%L
\frac{\beta_{0}+n_{c_{i}}^{a_{i}}}{4\beta_{0}+n_{a_{i}}}%C
}%分子
{\sum_{c'_{i}}\prod_{F}\frac{\gamma_{0}+n^{F, c'_{i}}_{s_{i}}}{2r_{0}+n^{F}_{c'_{i}}}%S
\frac{\eta_{0}+n_{l_{i}}^{c'_{i}}}{2\eta_{0}+n_{c'_{i}}}%L
\frac{\beta_{0}+n_{c'_{i}}^{a_{i}}}{4\beta_{0}+n_{a_{i}}} %C
}%分母
\end{split}
\end{equation}
%\end{comment}

\subsection{Pseudo-code for Gibbs Sampling}

Input: speech acts $a_{k}$ and values of $\vec{S_{k}}$ for each utterance\\
Output: clause type assignment $c_{k}$ and counts $n_{c_{i}}, n_{s_{i}}$\\
Initialization: randomly assign values to $c$\\
For each iteration, do:  
\begin{enumerate}
\item For each $i$ from range $(0,N)$, do:
\item speechact $\leftarrow$ $a[i]$
\item clausetype$\leftarrow$ $c[i]$ 
%\item synfeatures$\leftarrow$ $\vec{S}[i]$ 
\item For each value $k$ of $c$, do:
$n_{c_{i}} -= 1$, $n^{k}_{c_{i}} -=1$
\begin{enumerate}
\item For each feature $f$ from range$(0, (|\vec{S}|)$:
\begin{enumerate}
\item $n_{c_{i}^{f}} -= 1$, $n_{s_{i}^{f}} -= 1$
\item calculate  $p(c_{i}| c_{-i}, \vec{a}, \vec{S_{i}}, \beta )$ with equation (\ref{postC})
\item clausetype $\leftarrow$ sample from $ p(c_{i}| c_{-i}, \vec{a}, \vec{S_{i}}, \beta )$
\item $c[i]\leftarrow$ clausetype
\item $n_{c_{i}^{f}} += 1$, $n_{s_{i}^{f}} += 1$
\end{enumerate}
\item $n_{c_{i}} += 1$, $n^{k}_{c_{i}} +=1$
\end{enumerate}
\item return $c, n_{c}, n_{s}$
\end{enumerate}





